code/ecdsa/Hacl.Impl.EC.P521.Reduction.fst
@@ -1,0 +1,9 @@
+module Hacl.Impl.EC.P521.Reduction
+
+(* INPUT: An integer c = (c1041,..., c2, c1, c0) in base 2 with 0 ≤ c < p2
+521.
+OUTPUT: c mod p521.
+1. Define 521-bit integers:
+s1 = (c1041,..., c523, c522, c521),
+s2 = (c520,..., c2, c1, c0).
+2. Return(s1 +s2 mod p521). *)
